Started prototyping symbolized terms in Coq

Induction.v
@@ -57,26 +57,139 @@ Definition EveryInductiveNaturalIsInductive : ∀ n, InductiveNaturalIsInductive
      
  ). *)
  
- Definition ChurchTerm := ∀ (P : Prop),
+ 
+ 
+Definition ChurchNaturalT := ∀(P : Type) ,(P → P) → P →P.
+Definition ChurchNaturalTLower : ChurchNaturalT → ChurchNatural := λ n, n ChurchNatural churchSuccessor churchZero.
+Definition churchZeroT : ChurchNaturalT := λ _ _ p , p.
+Definition churchSuccessorT : ChurchNaturalT → ChurchNaturalT := λ predecessor P f p ,f (predecessor P f p).
+Eval cbv in ChurchNaturalTLower.
+Definition GenericNaturalIsInductiveT := λ(Natural : Type)(zero : Natural)(successor : Natural → Natural)(n : Natural),∀ (P : Natural →Type) (zeroCase :P zero)(successorCase :∀ (m : Natural) ,P m →P (successor m)),P n.
+
+Definition ChurchNaturalIsInductiveT := GenericNaturalIsInductiveT ChurchNaturalT churchZeroT churchSuccessorT.
+ (* λ(n : ChurchNatural),∀ (P : ChurchNatural →Prop) (zeroCase :P churchZero)(successorCase :∀ (m : ChurchNatural) ,P m →P (churchSuccessor m)),P n. *)
+Definition churchZeroIsInductiveT : ChurchNaturalIsInductiveT churchZeroT:= (λ _ zeroCase _, zeroCase).
+Definition churchSuccessorIsInductiveT : ∀(n : ChurchNaturalT), ChurchNaturalIsInductiveT n →ChurchNaturalIsInductiveT (churchSuccessorT n):= λ n nIsInductive, (λ P zeroCase successorCase, successorCase n (nIsInductive P zeroCase successorCase)).
+
+Definition ExistentialT :=λ(T : Type)(P :T → Type), ∀ (C : Type),(∀(t : T),P t→ C) → C.
+Definition ExistentialConstructorT :=λ(T : Type)(P :T → Type)(t : T) (p : P t)(C : Type)(consumer :(∀(t : T),P t→ C) ), consumer t p.
+
+Definition nargs : ∀ (n : ChurchNaturalT), Type := λ n, n Prop (λ (thingy : Prop) , (∀ (A : True), thingy)) True.
+Eval cbv in (nargs churchZeroT).
+Definition nargs_val : ∀ (n : ChurchNaturalT), ChurchNaturalIsInductiveT n → nargs n := λ n nIsInductive,
+  nIsInductive nargs I (λ m (thingy : nargs m) , (λ (A : True), thingy)).
+
+Eval cbv in (nargs (λ(P : Type) r p, r (r (r (r (r p)))))).
+Eval cbv in (nargs_val 
+  (churchSuccessorT (churchSuccessorT churchZeroT))
+  (churchSuccessorIsInductiveT (churchSuccessorT churchZeroT) (churchSuccessorIsInductiveT churchZeroT churchZeroIsInductiveT))
+).
+Eval cbv in nargs.
+ 
+ Definition Term : Type := ∀ (P : Type),
    ∀ (PropReduce : P) ,
    ∀ (TypeReduce : P) ,
+   ∀ (VarReduce : P) ,
    ∀ (PopReduce : P → P) ,
    ∀ (LambdaReduce : P → P → P) ,
    ∀ (ForAllReduce : P → P → P) ,
    ∀ (ApplyReduce : P → P → P) ,
    P.
-Definition churchProp : ChurchTerm := λ p pr t po l f a , pr.
-Definition churchApply : ChurchTerm → ChurchTerm → ChurchTerm := λ m n p pr t po l f a , a (m p pr t po l f a) (n p pr t po l f a) .
+Definition prop : Term := λ p pr t v po l f a , pr.
+Definition type : Term := λ p pr t v po l f a , t.
+Definition var : Term := λ p pr t v po l f a , v.
+Definition pop : Term → Term := λ m p pr t v po l f a , po (m p pr t v po l f a).
+Definition lambda : Term → Term → Term := λ m n p pr t v po l f a , l (m p pr t v po l f a) (n p pr t v po l f a) .
+Definition forAll : Term → Term → Term := λ m n p pr t v po l f a , f (m p pr t v po l f a) (n p pr t v po l f a) .
+Definition apply : Term → Term → Term := λ m n p pr t v po l f a , a (m p pr t v po l f a) (n p pr t v po l f a) .
 
-Definition InductiveTerm := λ (t : ChurchTerm) , ∀ (P : ChurchTerm → Prop) ,
-   ∀ (PropReduce : P churchProp) ,
-   ∀ (TypeReduce : P) ,
-   ∀ (PopReduce : P) ,
-   ∀ (LambdaReduce : P) ,
-   ∀ (ForAllReduce : P) ,
-   ∀ (ApplyReduce : ∀(m n : ChurchTerm), P (churchApply m n)) ,
+Definition TermIsInductive : Term → Prop := λ (t : Term) , ∀ (P : Term → Prop) ,
+   ∀ (PropReduce : P prop) ,
+   ∀ (TypeReduce : P type) ,
+   ∀ (VarReduce : P var) ,
+   ∀ (PopReduce : ∀(m : Term) , P m → P (pop m)) ,
+   ∀ (LambdaReduce : ∀(m n : Term), P m → P n → P (lambda m n)) ,
+   ∀ (ForAllReduce : ∀(m n : Term), P m → P n → P (forAll m n)) ,
+   ∀ (ApplyReduce : ∀(m n : Term), P m → P n → P (apply m n)) ,
+   P t.
+   
+Definition propIsInductive : TermIsInductive prop := λ p pr t v po l f a , pr.
+Definition typeIsInductive : TermIsInductive type := λ p pr t v po l f a , t.
+Definition varIsInductive : TermIsInductive var := λ p pr t v po l f a , v.
+Definition popIsInductive : ∀(m : Term),
+  TermIsInductive m → TermIsInductive (pop m) := 
+  λ m mi p pr t v po l f a , po m (mi p pr t v po l f a).
+Definition lambdaIsInductive : ∀(m n : Term),
+  TermIsInductive m → TermIsInductive n → TermIsInductive (lambda m n) := 
+  λ m n mi ni p pr t v po l f a , l m n (mi p pr t v po l f a) (ni p pr t v po l f a).
+Definition forAllIsInductive : ∀(m n : Term),
+  TermIsInductive m → TermIsInductive n → TermIsInductive (forAll m n) := 
+  λ m n mi ni p pr t v po l f a , f m n (mi p pr t v po l f a) (ni p pr t v po l f a).
+Definition applyIsInductive : ∀(m n : Term),
+  TermIsInductive m → TermIsInductive n → TermIsInductive (apply m n) := 
+  λ m n mi ni p pr t v po l f a , a m n (mi p pr t v po l f a) (ni p pr t v po l f a).
+
+Definition Context : Prop := ∀ (P : Prop),
+   ∀ (NilReduce : P) ,
+   ∀ (ConsReduce : Term → P → P) ,
    P.
-  
+
+Definition emptyContext : Context := λ _ n _, n.
+Definition consContext : Term → Context → Context := λ h t p n c, c h (t p n c).
+   
+ Definition TypeJudgmentT : Context → Term → Prop := λ context valueTerm typeTerm ,
+   ∀ (∀ (PropReduce : P emptyContext prop type → Type) ,
+   ∀ (∀ (TypeReduce : P) ,
+   ∀ (∀ (PopReduce : P → P) ,
+   ∀ (∀ (LambdaReduce : P → P → P) ,
+   ∀ (∀ (ForAllReduce : P → P → P) ,
+   ∀ (∀ (ApplyReduce : P → P → P) ,
+   → Type.
+
+Definition TypeJudgmentTIsInductive : ∀(c:Context)(t:Term), TypeJudgmentT c t → Type := λ (t : Term) , ∀ (P : Term → Type) ,
+   ∀ (PropReduce : P prop) ,
+   ∀ (VarReduce : P var) ,
+   ∀ (PopReduce : ∀(m : Term) , P m → P (pop m)) ,
+   ∀ (ForAllReduce : ∀(m n : Term), P m → P n → P (forAll m n)) ,
+   ∀ (ApplyReduce : ∀(m n : Term), P m → P n → P (apply m n)) ,
+   P t.
+   
+Definition propJudgment : TypeJudgment emptyContext prop type := .
+
+Definition interpretT : ∀(c:Context)(t:Term), TermIsInductive t → Judgment c t type → Type := λ context term judgment ,
+  judgment
+    
+    (λ ??, Prop)
+    
+    (λ (A : Prop), A → type)
+    (λ (A : Type), A → type).
+    
+    
+    
+    (λ (A : Prop), A → B)
+    (λ (A : Type) (B : Type), A → B)
+    (λ , ∀ (a : A), B)
+    (λ , ∀ (a : A), type)
+    (λ , ∀ (a : A), B)
+    
+    .
+interpret : ∀(c:Context)(t:Term)(ty:Term), (ty != TermT) -> (Judgment c t ty) -> ∃(A:T),A
+
+
+Definition nargs : ∀ (n : ChurchNatural), Prop := λ n, n Prop (∀ (thingy : Prop) , (∀ (A : True), thingy)) True. 
+
+
+Definition Weird : ∀ (q : bool), match q with
+| true => True
+| false => ~ False
+end := λ q , match q with
+| true => I
+| false => λ f, f
+end.
+
+Lemma Foo: True.
+  refine (Weird true).
+  refine (_ _).
 
 
 
